# 习题7.1

## 4

若$f$是可逆元，其逆为$g$。

由$fg=1$有$\deg(fg)=\deg(1)=0$。又由$\deg(fg)=\deg(f)+\deg(g)$，知$\deg(f)+\deg(g)=0$。由于$\forall f,\deg(f)\in\{-\infty\}\cup\mathbb N$，知$\deg(f)=0$。$\blacksquare$

## 5

设$a$是可逆元，$b=a^{-1}$。

若$ac=0$，则$c=(a^{-1}a)c=a^{-1}(ac)=0$。故没有非零$c$使$ac=0$，故$a$不是左零因子。对右零因子也成立。$\blacksquare$

## 6

1. 若$b=0$，则$A^{-1}=I$。

2. 若$b\ne0$，由于$K$是数域，$b\in K$，故$b^{-1}$存在。对$(A|I)$进行初等列变换成为$(I|B)$，知
   $$
   A^{-1}=B = \begin{pmatrix}
   	1 & -\frac{1}{b} & -\frac{1}{b^2} & \cdots & -\frac{1}{b^{n-2}} & -\frac{1}{b^{n-1}} \\
   	0 & 1 & -\frac{1}{b} & \cdots & -\frac{1}{b^{n-3}} & -\frac{1}{b^{n-2}} \\
   	\vdots & \vdots & \vdots & & \vdots & \vdots \\
   	0 & 0 & 0 & \cdots & 1 & -\frac{1}{b} \\
   	0 & 0 & 0 & \cdots & 0 & 1
   \end{pmatrix}
   $$
   

## 7

$$
|\lambda I-kA|=k^n|\frac{\lambda}{k}I-A|
$$

将$\lambda'=\frac{1}{k}\lambda$代入$|\lambda' I - A|=\prod_i(\lambda'-\lambda_i)^{l_i}$，有
$$
|\frac{\lambda}{k}I-A| = |\lambda' I - A|=\prod_i(\lambda'-\lambda_i)^{l_i}
$$
因此，
$$
k^n|\frac{\lambda}{k}I-A|=k^n\prod_i(\lambda'-\lambda_i)^{l_i}=\prod_i(\lambda-k\lambda_i)^{l_i}
$$
得证。$\blacksquare$

## 9

由对称性，只需证一边。下证$0a=0$：
$$
\begin{aligned}
0 &= 0+0 \\
0a &= (0+0)a \\
0a + (-0a) &= (0a + 0a) + (-0a) \\
0 &= 0a &\blacksquare
\end{aligned}
$$

## 10

先证$a(-b)=-ab$。
$$
\begin{aligned}
 b + (-b) &= 0 \\
 a(b + (-b)) &= 0 \\
 ab + a(-b) &= 0 \\
 a(-b) &= -ab
\end{aligned}
$$
$(-a)b=-ab$类似可证。

最后证$(-a)(-b)=ab$：
$$
\begin{aligned}
 (-a)(-b) &= -((-a)b) \\
  &= -(-ab)
\end{aligned}
$$
只需证$-(-ab)=ab$：
$$
\begin{aligned}
 -(-ab) + (-ab) &= ab + (-ab) \\
 -(-ab) &= ab & (消去(-ab))
\end{aligned}
$$
得证。$\blacksquare$

# 习题7.2

## 2

设$f_i(x)=h_i(x)g(x)$，有
$$
\begin{aligned}
\sum_i u_i(x)f_i(x) &= \sum_{i} u_i(x)(h_i(x)g(x)) \\
 &= \sum_{i} (u_i(x)h_i(x))g(x) \\
 &= \left(\sum_{i} u_i(x)h_i(x)\right)g(x)
\end{aligned}
$$
故
$$
g(x) \mid \sum_i u_i(x)f_i(x)
$$

## 3(2)

$$
x^4+x^3-2x+3=\boxed{\left(\frac{x^2}{3}+\frac{4x}{9}-\frac{2}{27}\right)}(3x^2-x+2) + \boxed{\frac{85}{27}-\frac{80x}{27}}
$$

## 4

$$
x^4-3x^3+a_1x+a_0=(x^2-1)(x^2-3x+1)+(a_1-3)x+(a_0+1)
$$

由$g(x)|f(x)$知
$$
g(x)|f(x)-(x^2-1)g(x)=(a_1-3)x+(a_0+1)
$$
又$\deg{g}=2>1\ge \deg((a_1-3)x+(a_0+1))$，知$a_1=3,a_0=-1$。$\blacksquare$

## 7

先证在$K[x]$中有
$$
(x^m-a^m)=(x-a)(x^{m-1}a^0+\cdots+x^0a^{m-1})
$$
证明：
$$
\begin{aligned}
(x-a)\sum_{i=0}^{m-1}x^{m-1-i}a^i &= \sum_{i=0}^{m-1}x^{m-i}a^i - \sum_{i=0}^{m-1}x^{m-1-i}a^{i+1} \\
 &= \sum_{i=0}^{m-1}x^{m-i}a^i - \sum_{i=1}^{m}x^{m-i}a^{i} \\
 &= x^m -a^m
\end{aligned}
$$
由此
$$
(x-a)|(x^m-a^m)
$$
商式为
$$
a^0x^{m-1}+\cdots+a^{m-1}x^0
$$


## 8

$$
(x^{2m+1}+a^{2m+1})=(x+a)\boxed{\sum_{i=0}^{2m}(-1)^ix^ia^{2m-i}}
$$

证明：
$$
\begin{aligned}
 (x+a)\sum_{i=0}^{2m}(-1)^ix^ia^{2m-i} &= \sum_{i=0}^{2m}(-1)^ix^{i+1}a^{2m-i} + \sum_{i=0}^{2m}(-1)^ix^{i}a^{2m+1-i} \\
 &= \sum_{i=1}^{2m+1}(-1)^{i+1}x^{i}a^{2m+1-i} + \sum_{i=0}^{2m}(-1)^ix^{i}a^{2m+1-i} \\
 &= -\sum_{i=1}^{2m+1}(-1)^{i}x^{i}a^{2m+1-i} + \sum_{i=0}^{2m}(-1)^ix^{i}a^{2m+1-i} \\
 &= -(-1)^{2m+1}x^{2m+1}a^0+(-1)^0x^0a^{2m+1} \\
 &= x^{2m+1}+a^{2m+1}
\end{aligned}
$$
